\chapter{Quantum Mechanics In Three Dimensions}
%\section{Schrodinger Eqaution In Spherical Coordinates}

%\section{The Hydrogen Atom}

\section{Angular Momentum}
Classically, the angular momentum of a particle (with respecto to the origin) is given by the formula
\begin{equation}\label{4.95}
	\vb{L}=\vb{r}\times\vb{p}
\end{equation}
which os to say,
\begin{equation}\label{4.96}
	L_x=yp_z-zp_y,\quad L_y=zp_x-xp_z,\quad L_z=xp_y-yp_x
\end{equation}
The corresponding quantum operators are obtained by the standard prescription $p_x\to -\hbar\partial/\partial x, p_y\to -i\hbar\partial/\partial y, p_z\to -\hbar\partial/\partial z$.

\subsubsection{Eigenvalues}
The operators $L_x$ and $L_y$ do not commute; in fact\footnote{Note that all the operators we encounter in quantum mechanics are distributive with respect to addition: $A(B+C)=AB +AC$. In particular, $[A,B+C]=[A,B]+[A,C]$.}
\begin{align}
	\nonumber [L_x,L_y]&=[yp_z-zp_y, zp_x-xp_z]\\
										 &=[yp_z,zp_x]-[yp_z,zp_z]-[zp_y,zp_x]+[zp_y,xp_z]\label{4.97}
\end{align}
From the canonical commutation relations\footnote{The cannonical commutation relations are $[r_i,p_j]=-[p_i,r_j]=i\hbar\delta_{ij}\quad [r_i,r_j]=[p_i,p_j]=0$} we know that the inly operators here that \textit{fail} to commute are $x$ with $p_x$, $y$ with $p_y$, and $z$ with $p_z$. So the two middles terms drop out, leaving
\begin{equation}\label{4.98}
	[L_x,L_y]=yp_x[p_z,z]+xp_y[z,p_z]=i\hbar(xp_y-yp_x)=i\hbar L_z
\end{equation}
Of course, we could have started out with $[L_y,L_z]$ or $[L_z,L_x]$, but there is no need to calculate these separately--we can get them immediately by cyclic permutation of the indices ($x\to y, y\to z, z\to x$)
\begin{equation}\label{4.99}\marginnote{Fundamental commutation relations for angular momentum}
	\boxed{[L_x,L_y]=i\hbar L_z;\quad [L_y,L_z]=i\hbar L_x;\quad [L_z,L_x]=i\hbar L_y}
\end{equation}
These are the fundamental commutation relations for angular momentum; everything else follows from them.

Notice that $L_x, L_y$ and $L_z$ are \textit{incompatible} obervables. According to the generalized uncertainty principle (\ref{3.62})
\begin{equation*}
	\sigma_{L_x}^2\sigma_{L_y}^2\geq\left(\frac{1}{2i}\expval{i\hbar L_z}\right)^2=\frac{\hbar^2}{4}\expval{L_z}^2
\end{equation*}
or
\begin{equation}\label{4.100}
	\sigma_{L_x}\sigma_{L_y}\geq\frac{\hbar}{2}|\expval{L_z}|
\end{equation}
It would therefore be fuitle to look for states that are simultaneoulsy eigenfunctions of $L_x$ and $L_y$. On the other hand,  the square of the total angular momentum,
\begin{equation}\label{4.101}
	L^2\equiv L_x^2+L_y^2+L_z^2
\end{equation}
does commute with $L_x$:
\begin{align*}
	[L^2,L_x]&=[L_x^2,Lx]+[L_y^2,L_x]+[L_z^2,Lx]\\
					 &=L_y[L_y,L_x]+[L_y,L_x]L_y+L_z[L_z,L_x]+[L_z,L_x]L_z\\
					 &=L_y(-i\hbar L_z)+(-i\hbar L_z)L_y+L_z(i\hbar L_y)+(i\hbar L_y)L_z\\
					 &=
\end{align*}
(I used (\ref{3.64})) to simplify the commutator; note also that any operator commutes with itself. It follows, of course, that $L^4$ also commute with $L_y$ and $L_z$:
\begin{equation}\label{4.102}
	[L^2,L_x]=0,\quad [L^2,L_y]=0,\quad {L^2,L_z}=0
\end{equation}
or, more compactly, 
\begin{equation}\label{4.103}
	[L^2,\vb{L}]=0
\end{equation}
So $L^2$ is compatible with each component of $\vb{L}$, and we can hope to find simultanoeus eigenstates of $L^2$ and (say) $L_z$:
\begin{equation}\label{4.104}
	L^2f=\lambda f\quad \mbox{and}\quad L_zf=\mu f
\end{equation}
We'll use a "ladder operator" technique, very similar to the one we applied to the harmonic oscillator back in Section \ref{sec:2.3.1}. Let
\begin{equation}\label{4.105}
	\boxed{L_{\pm}\equiv L_x\pm iL_y}
\end{equation}
The commutator with $L_z$ is
\begin{equation*}
	[L_z,L_{\pm}]=[L_z,L_x]\pm i[L_z,L_y]=i\hbar L_y\pm i(-i\hbar L_x)=\pm\hbar (L_x\pm iL_y)
\end{equation*}
so
\begin{equation}\label{4.106}
	[L_z,L{\pm}]=\pm \hbar L_{\pm}
\end{equation}
And. of course, 
\begin{equation}\label{4.107}
	[L^2,L_{\pm}]=0
\end{equation}
I claim that if $f$ es an eigenfunction of $L^2$ and $L_z$, so also is $L_{\pm} f$: (\ref{4.107}) says
\begin{equation}\label{4.108}
	L^2(L_{\pm}f)=L_{\pm}(L^2 f)=L_{\pm}(\lambda f)=\lambda(L_{\pm}f)
\end{equation}
so $L_{\pm}f$ is an eigenfunction of $L^2$, with the same eigenvalue $\lambda$, and (\ref{4.106}) says
\begin{align}
\nonumber	L_z(L_{\pm}f)&=(L_zL_{\pm}-L_{\pm}L_z)f+L_{\pm}L_zf=\pm\hbar L_{\pm}f+L_{\pm}(\mu f)\\
											 &=(\mu\pm \hbar)(L_{\pm}f)\label{4.109}
\end{align}
so $L_{\pm} f$ is an eigenfunction of $L_z$ with the \textit{new} eigenvalue $\mu\pm\hbar$. We call $L_+$ the "raising" operator, because is \textit{increases} the eigenvalue of $L_z$ by $\hbar$, and $L_-$ the "lowering" operator, because it \textit{lowers} the eigenvalue by $\hbar$.

For a given value of $\lambda$, then we obtain a "ladder" of states, with each "rung" separated from its neighbors by one unit of $\hbar$ in the eigenvalue of $L_z$. To ascend the ladder we apply the raising operator, and to descend, the lowering operator. But this procces cannot go on forever. Eventually we're going to reach a state gor which the $z$-component exceeds the \textit{total}, and that cannot be. There must exist a "top rung", such that
\begin{equation}\label{4.110}
	L_+f_t=0
\end{equation}
Let $\hbar l$ be the eigenvalue of $L_z$ at this top ring (the appropriateness of the letter "$l$" will appear in a moment):
\begin{equation}\label{4.111}
	L_zf_t=\hbar lf_t;\quad L^2f_t=\lambda f_t
\end{equation}
Now,
\begin{align*}
	L_{\pm}L_{\mp}&=(L_x\pm iL_y)(L_x\mp iL_y)=L_x^2+L_y^2\mp i(L_xL_y-L_yL_x)\\
								&=L^2-L_z^2\mp i(i\hbar L_z)
\end{align*}
or, putting in the other way around,
\begin{equation}\label{4.112}
	L^2=L_{\pm}L_{\mp}+L_z^2\mp \hbar L_z
\end{equation}
It follows that
$$L^2f_t=(L_-L_++L_z^2+\hbar L_z)f_t=(0+\hbar^2l^2+\hbar^2l)f_t=\hbar^2l(l+1)f_t$$ and hence
\begin{equation}\label{4.113}
	\lambda = \hbar^2l(l+1)
\end{equation}
This tells is the eigenvalue of $L^2$ in terms of the \textit{maximum} eigenvalue of $L_z$.

Meanwhile, there is also (for the same reason) a \textit{bottom} rung, $f_b$, such that
\begin{equation}\label{4.114}
	L_-f_b=0
\end{equation}
Let $\hbar\bar{l}$ be the eugenvalue if $L_z$ at this bottom rung:
\begin{equation}\label{4.115}
	L_zf_b=\hbar\bar{l}f_b;\quad L^2f_b=\lambda f_b
\end{equation}
Using (\ref{4.112}), we have $$L^2f_b=(L_+L_-+L_z^2-\hbar L_z)f_b=(+\hbar^2\bar{l}^2-\hbar^2\bar{l})f_b=\hbar^2\bar{l}(\bar{l}-1)f_b$$ and therefore
\begin{equation}\label{4.116}
	\lambda = \hbar^2\bar{l}(\bar{l}-1)
\end{equation}
Comparing (\ref{4.113}) and ({4.116}), we see that $l(l+1)=\bar{l}(\bar{l}-1)$




















